src/QL/FOL/Tait/tait.lean
@@ -1,39 +1,43 @@
-import QL.FOL.deduction QL.FOL.language QL.FOL.uniform
+import QL.FOL.coding
 
 universes u v
 
 namespace fol
 open_locale logic_symbol aclogic
-open subformula
-variables (L L₁ L₂ : language.{u}) (m m₁ m₂ n : ℕ)
+
+variables (L L₁ L₂ : language.{u}) (μ : Type v) (μ₁ : Type*) (μ₂ : Type*) (m m₁ m₂ n : ℕ)
 
 namespace Tait
 
-inductive subformula (m) : ℕ → Type u
+inductive subformula (μ : Type v) : ℕ → Type (max u v)
 | verum        {n} : subformula n
 | falsum       {n} : subformula n
-| relation     {n} : ∀ {p}, L.pr p → (fin p → subterm L m n) → subformula n
-| neg_relation {n} : ∀ {p}, L.pr p → (fin p → subterm L m n) → subformula n
+| relation     {n} : ∀ {p}, L.pr p → (fin p → subterm L μ n) → subformula n
+| neg_relation {n} : ∀ {p}, L.pr p → (fin p → subterm L μ n) → subformula n
 | and          {n} : subformula n → subformula n → subformula n
 | or           {n} : subformula n → subformula n → subformula n
 | fal          {n} : subformula (n + 1) → subformula n
 | ex           {n} : subformula (n + 1) → subformula n
 
-@[reducible] def formula (m) := subformula L m 0
+@[reducible] def formula := subformula L μ 0
 
-@[reducible] def sentence := formula L 0
+@[reducible] def bounded_subformula (m n : ℕ) := subformula L (fin m) n
 
-variables {L m n}
+@[reducible] def bounded_formula (m : ℕ) := bounded_subformula L m 0
+
+@[reducible] def sentence := bounded_formula L 0
+
+variables {L μ n}
 
 namespace subformula
 
-instance : has_univ_quantifier' (subformula L m) := ⟨@fal L m⟩
+instance : has_univ_quantifier' (subformula L μ) := ⟨@fal L μ⟩
 
-instance : has_exists_quantifier' (subformula L m) := ⟨@ex L m⟩
+instance : has_exists_quantifier' (subformula L μ) := ⟨@ex L μ⟩
 
 attribute [pattern]  has_sup.sup has_inf.inf has_univ_quantifier.univ has_exists_quantifier.ex
 
-@[simp] def not : ∀ {n}, subformula L m n → subformula L m n
+@[simp] def not : ∀ {n}, subformula L μ n → subformula L μ n
 | n verum              := falsum
 | n falsum             := verum
 | n (relation r v)     := neg_relation r v
@@ -43,49 +47,48 @@ attribute [pattern]  has_sup.sup has_inf.inf has_univ_quantifier.univ has_exists
 | n (fal p)            := ex (not p)
 | n (ex p)             := fal (not p)
 
-def imply (p q : subformula L m n) := or (not p) q
+def imply (p q : subformula L μ n) := or (not p) q
 
-instance : has_logic_symbol (subformula L m n) := Tait.logic_simbol_default (subformula L m n) verum falsum not and or
+instance : has_logic_symbol (subformula L μ n) := Tait.logic_simbol_default (subformula L μ n) verum falsum not and or
+ 
+lemma verum_eq : @verum L μ n = ⊤ := rfl
+lemma falsum_eq : @falsum L μ n = ⊥ := rfl
+lemma and_eq : @and L μ n = has_inf.inf := rfl
+lemma or_eq : @or L μ n = has_sup.sup := rfl
+lemma not_eq : @not L μ n = has_negation.neg := rfl
+lemma imply_eq : @imply L μ n = has_arrow.arrow := rfl
+lemma imply_def (p q : subformula L μ n) : (p ⟶ q) = (∼p) ⊔ q := by simp[←imply_eq, imply]; refl
+lemma fal_eq : @fal L μ n = has_univ_quantifier'.univ := rfl
+lemma ex_eq : @ex L μ n = has_exists_quantifier'.ex := rfl
 
-lemma verum_eq : @verum L m n = ⊤ := rfl
-lemma falsum_eq : @falsum L m n = ⊥ := rfl
-lemma and_eq : @and L m n = has_inf.inf := rfl
-lemma or_eq : @or L m n = has_sup.sup := rfl
-lemma not_eq : @not L m n = has_negation.neg := rfl
-lemma imply_eq : @imply L m n = has_arrow.arrow := rfl
-lemma imply_def (p q : subformula L m n) : (p ⟶ q) = (∼p) ⊔ q := by simp[←imply_eq, imply]; refl
-lemma fal_eq : @fal L m n = has_univ_quantifier'.univ := rfl
-lemma ex_eq : @ex L m n = has_exists_quantifier'.ex := rfl
-
-
-@[simp] lemma and.inj' (p₁ q₁ p₂ q₂ : subformula L m n) : p₁ ⊓ p₂ = q₁ ⊓ q₂ ↔ p₁ = q₁ ∧ p₂ = q₂ :=
+@[simp] lemma and.inj' (p₁ q₁ p₂ q₂ : subformula L μ n) : p₁ ⊓ p₂ = q₁ ⊓ q₂ ↔ p₁ = q₁ ∧ p₂ = q₂ :=
 by simp[has_inf.inf]
 
-@[simp] lemma or.inj' (p₁ q₁ p₂ q₂ : subformula L m n) : p₁ ⊔ p₂ = q₁ ⊔ q₂ ↔ p₁ = q₁ ∧ p₂ = q₂ :=
+@[simp] lemma or.inj' (p₁ q₁ p₂ q₂ : subformula L μ n) : p₁ ⊔ p₂ = q₁ ⊔ q₂ ↔ p₁ = q₁ ∧ p₂ = q₂ :=
 by simp[has_sup.sup]
 
-@[simp] lemma fal.inj' (p q : subformula L m (n + 1)) : (∀'p : subformula L m n) = ∀'q ↔ p = q := ⟨fal.inj, congr_arg _⟩
+@[simp] lemma fal.inj' (p q : subformula L μ (n + 1)) : ∀'p = ∀'q ↔ p = q := ⟨fal.inj, congr_arg _⟩
 
-@[simp] lemma ex.inj' (p q : subformula L m (n + 1)) : (∃'p : subformula L m n) = ∃'q ↔ p = q := 
+@[simp] lemma ex.inj' (p q : subformula L μ (n + 1)) : ∃'p = ∃'q ↔ p = q := 
 by simp[has_exists_quantifier'.ex]
 
-@[simp] lemma not_falsum : ∼(⊥ : subformula L m n) = ⊤ := rfl
+@[simp] lemma not_falsum : ∼(⊥ : subformula L μ n) = ⊤ := rfl
 
-@[simp] lemma not_verum : ∼(⊤ : subformula L m n) = ⊥ := rfl
+@[simp] lemma not_verum : ∼(⊤ : subformula L μ n) = ⊥ := rfl
 
-@[simp] lemma not_relation {k} (r : L.pr k) (v : fin k → subterm L m n) : ∼(relation r v) = neg_relation r v := rfl
+@[simp] lemma not_relation {k} (r : L.pr k) (v : fin k → subterm L μ n) : ∼(relation r v) = neg_relation r v := rfl
 
-@[simp] lemma not_neg_relation {k} (r : L.pr k) (v : fin k → subterm L m n) : ∼(neg_relation r v) = relation r v := rfl
+@[simp] lemma not_neg_relation {k} (r : L.pr k) (v : fin k → subterm L μ n) : ∼(neg_relation r v) = relation r v := rfl
 
-@[simp] lemma not_and (p q : subformula L m n) : ∼(p ⊓ q) = ∼p ⊔ ∼q := rfl
+@[simp] lemma not_and (p q : subformula L μ n) : ∼(p ⊓ q) = ∼p ⊔ ∼q := rfl
 
-@[simp] lemma not_or (p q : subformula L m n) : ∼(p ⊔ q) = ∼p ⊓ ∼q := rfl
+@[simp] lemma not_or (p q : subformula L μ n) : ∼(p ⊔ q) = ∼p ⊓ ∼q := rfl
 
-@[simp] lemma not_fal (p : subformula L m (n + 1)) : ∼(∀'p) = ∃'∼p := rfl
+@[simp] lemma not_fal (p : subformula L μ (n + 1)) : ∼(∀'p) = ∃'∼p := rfl
 
-@[simp] lemma not_ex (p : subformula L m (n + 1)) : ∼(∃'p) = ∀'∼p := rfl
+@[simp] lemma not_ex (p : subformula L μ (n + 1)) : ∼(∃'p) = ∀'∼p := rfl
 
-@[simp] def complexity : Π {n}, subformula L m n → ℕ
+@[simp] def complexity : Π {n}, subformula L μ n → ℕ
 | n verum              := 0
 | n falsum             := 0
 | n (relation r v)     := 0
@@ -95,23 +98,91 @@ by simp[has_exists_quantifier'.ex]
 | n (fal p)            := p.complexity + 1
 | n (ex p)             := p.complexity + 1
 
-section rew
-variables {m₁ m₂} (s : fin m₁ → subterm L m₂ n)
+def ind {C : Π n, subformula L μ n → Sort*}
+  (hverum : Π {n : ℕ}, C n ⊤)
+  (hfalsum : Π {n : ℕ}, C n ⊥)
+  (hrelation : Π {n l : ℕ} (r : L.pr l) (v : fin l → subterm L μ n), C n (relation r v))
+  (hneg_relation : Π {n l : ℕ} (r : L.pr l) (v : fin l → subterm L μ n), C n (neg_relation r v))
+  (hand : Π {n : ℕ} (p q : subformula L μ n), C n p → C n q → C n (p ⊓ q))
+  (hor : Π {n : ℕ} (p q : subformula L μ n), C n p → C n q → C n (p ⊔ q))
+  (hfal : Π {n : ℕ} (p : subformula L μ (n + 1)), C (n + 1) p → C n (∀'p))
+  (hex : Π {n : ℕ} (p : subformula L μ (n + 1)), C (n + 1) p → C n (∃'p)) :
+  Π {n : ℕ} (p : subformula L μ n), C n p
+| n verum              := hverum
+| n falsum             := hfalsum
+| n (relation r v)     := hrelation r v
+| n (neg_relation r v) := hneg_relation r v
+| n (and p q)          := hand p q (ind p) (ind q)
+| n (or p q)           := hor p q (ind p) (ind q)
+| n (fal p)            := hfal p (ind p)
+| n (ex p)             := hex p (ind p)
 
-@[simp] def rew' {m₁ m₂} : Π {n}, (fin m₁ → subterm L m₂ n) → subformula L m₁ n → subformula L m₂ n
-| n s verum              := ⊤
-| n s falsum             := ⊥
+--普通に帰納法をすると論理記号で表示されないから
+@[elab_as_eliminator]
+protected def ind_on {C : Π n, subformula L μ n → Sort*}
+  {n : ℕ} (p : subformula L μ n)
+  (verum : Π {n : ℕ}, C n ⊤)
+  (falsum : Π {n : ℕ}, C n ⊥)
+  (relation : Π {n l : ℕ} (r : L.pr l) (v : fin l → subterm L μ n), C n (relation r v))
+  (neg_relation : Π {n l : ℕ} (r : L.pr l) (v : fin l → subterm L μ n), C n (neg_relation r v))
+  (and : Π {n : ℕ} (p q : subformula L μ n), C n p → C n q → C n (p ⊓ q))
+  (or : Π {n : ℕ} (p q : subformula L μ n), C n p → C n q → C n (p ⊔ q))
+  (fal : Π {n : ℕ} (p : subformula L μ (n + 1)), C (n + 1) p → C n (∀'p))
+  (ex : Π {n : ℕ} (p : subformula L μ (n + 1)), C (n + 1) p → C n (∃'p)) :
+  C n p :=
+ind @verum @falsum @relation @neg_relation @and @or @fal @ex p
+
+def ind_succ {C : Π n, subformula L μ (n + 1) → Sort*}
+  (hverum : Π {n : ℕ}, C n ⊤)
+  (hfalsum : Π {n : ℕ}, C n ⊥)
+  (hrelation : Π {n l : ℕ} (r : L.pr l) (v : fin l → subterm L μ (n + 1)), C n (relation r v))
+  (hneg_relation : Π {n l : ℕ} (r : L.pr l) (v : fin l → subterm L μ (n + 1)), C n (neg_relation r v))
+  (hand : Π {n : ℕ} (p q : subformula L μ (n + 1)), C n p → C n q → C n (p ⊓ q))
+  (hor : Π {n : ℕ} (p q : subformula L μ (n + 1)), C n p → C n q → C n (p ⊔ q))
+  (hfal : Π {n : ℕ} (p : subformula L μ (n + 1 + 1)), C (n + 1) p → C n (∀'p))
+  (hex : Π {n : ℕ} (p : subformula L μ (n + 1 + 1)), C (n + 1) p → C n (∃'p)) :
+  Π {n : ℕ} (p : subformula L μ (n + 1)), C n p
+| n verum              := hverum
+| n falsum             := hfalsum
+| n (relation r v)     := hrelation r v
+| n (neg_relation r v) := hneg_relation r v
+| n (and p q)          := hand p q (ind_succ p) (ind_succ q)
+| n (or p q)           := hor p q (ind_succ p) (ind_succ q)
+| n (fal p)            := hfal p (ind_succ p)
+| n (ex p)             := hex p (ind_succ p)
+using_well_founded {rel_tac := λ _ _, `[exact ⟨_, measure_wf (λ x, x.2.complexity)⟩]}
+
+@[elab_as_eliminator]
+def ind_succ_on {C : Π n, subformula L μ (n + 1) → Sort*}
+  {n : ℕ} (p : subformula L μ (n + 1))
+  (verum : Π {n : ℕ}, C n ⊤)
+  (falsum : Π {n : ℕ}, C n ⊥)
+  (relation : Π {n l : ℕ} (r : L.pr l) (v : fin l → subterm L μ (n + 1)), C n (relation r v))
+  (neg_relation : Π {n l : ℕ} (r : L.pr l) (v : fin l → subterm L μ (n + 1)), C n (neg_relation r v))
+  (and : Π {n : ℕ} (p q : subformula L μ (n + 1)), C n p → C n q → C n (p ⊓ q))
+  (or : Π {n : ℕ} (p q : subformula L μ (n + 1)), C n p → C n q → C n (p ⊔ q))
+  (fal : Π {n : ℕ} (p : subformula L μ (n + 1 + 1)), C (n + 1) p → C n (∀'p))
+  (ex : Π {n : ℕ} (p : subformula L μ (n + 1 + 1)), C (n + 1) p → C n (∃'p)) :
+  C n p :=
+ind_succ @verum @falsum @relation @neg_relation @and @or @fal @ex p
+
+section rew
+variables {μ₁ μ₂} (s : μ₁ → subterm L μ₂ n) (f : μ₁ → μ₂)
+
+@[simp] def rew' {μ₁ μ₂} : Π {n}, (μ₁ → subterm L μ₂ n) → subformula L μ₁ n → subformula L μ₂ n
+| n s verum              := verum
+| n s falsum             := falsum
 | n s (relation p v)     := relation p (subterm.rew s ∘ v)
 | n s (neg_relation p v) := neg_relation p (subterm.rew s ∘ v)
-| n s (and p q)          := p.rew' s ⊓ q.rew' s
-| n s (or p q)           := p.rew' s ⊔ q.rew' s
-| n s (fal p)            := ∀'p.rew' (subterm.lift ∘ s)
-| n s (ex p)             := ∃'p.rew' (subterm.lift ∘ s)
+| n s (and p q)          := and (p.rew' s) (q.rew' s)
+| n s (or p q)           := or (p.rew' s) (q.rew' s)
+| n s (fal p)            := fal (p.rew' (subterm.lift ∘ s))
+| n s (ex p)             := ex (p.rew' (subterm.lift ∘ s))
 
-@[simp] lemma rew'_neg (p : subformula L m₁ n) : (∼p).rew' s = ∼(p.rew' s) :=
-by induction p; simp[mlift, ←verum_eq, ←falsum_eq, ←and_eq, ←or_eq, ←not_eq, ←fal_eq, ←ex_eq, *] at*
+@[simp] lemma rew'_neg (p : subformula L μ₁ n) : (∼p).rew' s = ∼(p.rew' s) :=
+by induction p; simp[←verum_eq, ←falsum_eq, ←and_eq, ←or_eq, ←not_eq, ←fal_eq, ←ex_eq, *] at*
 
-def rew (s : fin m₁ → subterm L m₂ n) : subformula L m₁ n →ₗ subformula L m₂ n :=
+def rew (s : μ₁ → subterm L μ₂ n) : subformula L μ₁ n →ₗ subformula L μ₂ n :=
 { to_fun := rew' s,
   map_neg' := λ p, by simp,
   map_imply' := λ p q, by simp[imply_def, ←or_eq],
@@ -120,82 +191,150 @@ def rew (s : fin m₁ → subterm L m₂ n) : subformula L m₁ n →ₗ subform
   map_top' := by refl,
   map_bot' := by refl }
 
-@[simp] lemma rew_relation {k} (r : L.pr k) (v : fin k → subterm L m₁ n) :
+def map (f : μ₁ → μ₂) : subformula L μ₁ n →ₗ subformula L μ₂ n := rew (λ x, &(f x))
+
+@[simp] lemma rew_relation {k} (r : L.pr k) (v : fin k → subterm L μ₁ n) :
   rew s (relation r v) = relation r (subterm.rew s ∘ v) := rfl
 
-@[simp] lemma rew_neg_relation {k} (r : L.pr k) (v : fin k → subterm L m₁ n) :
+@[simp] lemma rew_neg_relation {k} (r : L.pr k) (v : fin k → subterm L μ₁ n) :
   rew s (neg_relation r v) = neg_relation r (subterm.rew s ∘ v) := rfl
 
-@[simp] lemma rew_fal (p : subformula L m₁ (n + 1)) :
+@[simp] lemma rew_fal (p : subformula L μ₁ (n + 1)) :
   rew s (∀'p) = ∀'rew (subterm.lift ∘ s) p := rfl
 
-@[simp] lemma rew_ex (p : subformula L m₁ (n + 1)) :
+@[simp] lemma rew_ex (p : subformula L μ₁ (n + 1)) :
   rew s (∃'p) = ∃'rew (subterm.lift ∘ s) p := rfl
+
+@[simp] lemma map_relation {k} (r : L.pr k) (v : fin k → subterm L μ₁ n) :
+  map f (relation r v) = relation r (λ x, subterm.map f (v x)) := rfl
+
+@[simp] lemma map_neg_relation {k} (r : L.pr k) (v : fin k → subterm L μ₁ n) :
+  map f (neg_relation r v) = neg_relation r (λ x, subterm.map f (v x)) := rfl
+
+@[simp] lemma map_fal (p : subformula L μ₁ (n + 1)) :
+  map f (∀'p) = ∀'map f p := rfl
+
+@[simp] lemma map_ex (p : subformula L μ₁ (n + 1)) :
+  map f (∃'p) = ∃'map f p := rfl
+
+lemma eq_rew_of_eq {p : subformula L μ₁ n} {s₁ s₂ : μ₁ → subterm L μ₂ n} (h : s₁ = s₂) :
+  rew s₁ p = rew s₂ p := by rw[h]
+
+lemma eq_map_of_eq {p : subformula L μ₁ n} {f₁ f₂ : μ₁ → μ₂} (h : f₁ = f₂) :
+  map f₁ p = map f₂ p := by rw[h]
+
+lemma rew_rew {μ₁ μ₂ μ₃} : ∀ {n} (p : subformula L μ₁ n) (s₀ : μ₁ → subterm L μ₂ n) (s₁ : μ₂ → subterm L μ₃ n),
+  rew s₁ (rew s₀ p) = rew (λ x, subterm.rew s₁ (s₀ x)) p
+| n verum              s₀ s₁ := by simp[verum_eq]
+| n falsum             s₀ s₁ := by simp[falsum_eq]
+| n (relation p v)     s₀ s₁ := by simp; funext; simp[subterm.rew_rew]
+| n (neg_relation p v) s₀ s₁ := by simp; funext; simp[subterm.rew_rew]
+| n (and p q)          s₀ s₁ := by simp[and_eq, rew_rew p, rew_rew q]
+| n (or p q)           s₀ s₁ := by simp[or_eq, rew_rew p, rew_rew q]
+| n (fal p)            s₀ s₁ := by simp[fal_eq, rew_rew p]; refine eq_rew_of_eq (by funext x; simp[subterm.lift_rew])
+| n (ex p)             s₀ s₁ := by simp[ex_eq, rew_rew p]; refine eq_rew_of_eq (by funext x; simp[subterm.lift_rew])
+
+@[simp] lemma map_map {μ₁ μ₂ μ₃} (f₁ : μ₁ → μ₂) (f₂ : μ₂ → μ₃) (p : subformula L μ₁ n) :
+  map f₂ (map f₁ p) = map (f₂ ∘ f₁) p :=
+by simp[map, rew_rew]
+
+lemma map_inj_of_inj (f : μ₁ → μ₂) (I : function.injective f) :
+  function.injective (map f : Tait.subformula L μ₁ n → Tait.subformula L μ₂ n) := λ p q,
+begin
+  induction p,
+  case verum { cases q; simp[map, rew] },
+  case falsum { cases q; simp[map, rew] },
+  case relation : n k r v₁
+  { cases q; simp[map, rew],
+    case relation : _ _ r₂ v₂
+    { rintros rfl rfl, simp, intros h, funext i, exact subterm.map_inj_of_inj f I (congr_fun h i) } },
+  case neg_relation : n k r v₁
+  { cases q; simp[map, rew],
+    case neg_relation : _ _ r₂ v₂
+    { rintros rfl rfl, simp, intros h, funext i, exact subterm.map_inj_of_inj f I (congr_fun h i) } },
+  case and : n p₁ q₁ IH₁ IH₂ { cases q; simp[map, rew] at*, intros h₁ h₂, exact ⟨IH₁ _ h₁, IH₂ _ h₂⟩ },
+  case or : n p₁ q₁ IH₁ IH₂ { cases q; simp[map, rew] at*, intros h₁ h₂, exact ⟨IH₁ _ h₁, IH₂ _ h₂⟩ },
+  case fal : n p IH
+  { cases q; simp[map, rew],
+      case fal : _ p₂ { intros h, exact IH _ h } },
+  case ex : n p IH
+  { cases q; simp[map, rew],
+      case ex : _ p₂ { intros h, exact IH _ h } }
+end
 
 end rew
 
+section subst
+
+@[simp] def subst' : Π {n}, subterm L μ n → subformula L μ (n + 1) → subformula L μ n
+| n u verum              := ⊤
+| n u falsum             := ⊥
+| n u (relation r v)     := relation r (λ i, subterm.subst u $ v i)
+| n u (neg_relation r v) := neg_relation r (λ i, subterm.subst u $ v i)
+| n u (and p q)          := subst' u p ⊓ subst' u q
+| n u (or p q)           := subst' u p ⊔ subst' u q
+| n u (fal p)            := ∀' (subst' u.lift p)
+| n u (ex p)             := ∃' (subst' u.lift p)
+using_well_founded {rel_tac := λ _ _, `[exact ⟨_, measure_wf (λ x, x.2.2.complexity)⟩]}
+
+@[simp] lemma subst'_neg (p : subformula L μ₁ (n + 1)) : ∀ u, subst' u (∼p) = ∼(subst' u p) :=
+by apply ind_succ_on p; intros; simp[←verum_eq, ←falsum_eq, ←and_eq, ←or_eq, ←not_eq, ←fal_eq, ←ex_eq, *] at*
+
+def subst (u : subterm L μ n) : subformula L μ (n + 1) →ₗ subformula L μ n :=
+{ to_fun := subst' u,
+  map_neg' := λ p, by simp; refl,
+  map_imply' := λ p q, by simp[imply_def, ←or_eq],
+  map_and' := λ p q, by unfold has_inf.inf; simp; refl,
+  map_or' := λ p q, by unfold has_sup.sup; simp; refl,
+  map_top' := by unfold has_top.top; simp; refl,
+  map_bot' := by unfold has_bot.bot; simp; refl }
+
+variables (u : subterm L μ n)
+
+@[simp] lemma subst_relation {k} (r : L.pr k) (v : fin k → subterm L μ (n + 1)) :
+  subst u (relation r v) = relation r (λ i, u.subst (v i)) := by simp[subst]
+
+@[simp] lemma subst_neg_relation {k} (r : L.pr k) (v : fin k → subterm L μ (n + 1)) :
+  subst u (neg_relation r v) = neg_relation r (λ i, u.subst (v i)) := by simp[subst]
+
+@[simp] lemma subst_fal (p : subformula L μ (n + 1 + 1)) :
+  subst u (∀'p) = ∀'subst u.lift p := by simp[←fal_eq, subst]
+
+@[simp] lemma subst_ex (p : subformula L μ (n + 1 + 1)) :
+  subst u (∃'p) = ∃'subst u.lift p := by simp[←ex_eq, subst]
+
+variables {μ₁ μ₂} (f : μ₁ → μ₂)
+
+lemma map_subst (p : subformula L μ₁ (n + 1)) : ∀ (u : subterm L μ₁ n),
+  map f (subst u p) = subst (u.map f) (map f p) :=
+by apply ind_succ_on p; intros; simp[*, subterm.map_subst, subterm.map_lift]
+
+end subst
+
+section bounded
+variables {m}
+
 section mlift
 
-@[simp] def mlift' {m} : Π {n}, subformula L m n → subformula L (m + 1) n
-| n verum              := ⊤
-| n falsum             := ⊥
-| n (relation p v)     := relation p (subterm.mlift ∘ v)
-| n (neg_relation p v) := neg_relation p (subterm.mlift ∘ v)
-| n (and p q)          := p.mlift' ⊓ q.mlift'
-| n (or p q)           := p.mlift' ⊔ q.mlift'
-| n (fal p)            := ∀'p.mlift'
-| n (ex p)             := ∃'p.mlift'
+def mlift {m n} : bounded_subformula L m n →ₗ bounded_subformula L (m + 1) n := map fin.cast_succ
 
-@[simp] lemma mlift'_neg (p : subformula L m n) : (∼p).mlift' = ∼p.mlift' :=
-by induction p; simp[mlift, ←verum_eq, ←falsum_eq, ←and_eq, ←or_eq, ←not_eq, ←fal_eq, ←ex_eq, *] at*
-
-def mlift : subformula L m n →ₗ subformula L (m + 1) n :=
-{ to_fun := mlift',
-  map_neg' := λ p, by simp,
-  map_imply' := λ p q, by simp[imply_def, ←or_eq],
-  map_and' := λ p q, by refl,
-  map_or' := λ p q, by refl,
-  map_top' := by refl,
-  map_bot' := by refl }
-
-@[simp] lemma mlift_relation {k} (r : L.pr k) (v : fin k → subterm L m n) :
+@[simp] lemma mlift_relation {k} (r : L.pr k) (v : fin k → bounded_subterm L m n) :
   mlift (relation r v) = relation r (subterm.mlift ∘ v) := rfl
 
-@[simp] lemma mlift_neg_relation {k} (r : L.pr k) (v : fin k → subterm L m n) :
+@[simp] lemma mlift_neg_relation {k} (r : L.pr k) (v : fin k → bounded_subterm L m n) :
   mlift (neg_relation r v) = neg_relation r (subterm.mlift ∘ v) := rfl
 
-@[simp] lemma mlift_fal (p : subformula L m (n + 1)) :
+@[simp] lemma mlift_fal (p : bounded_subformula L m (n + 1)) :
   mlift (∀'p) = ∀'mlift p := rfl
 
-@[simp] lemma mslift_ex (p : subformula L m (n + 1)) :
+@[simp] lemma mslift_ex (p : bounded_subformula L m (n + 1)) :
   mlift (∃'p) = ∃'mlift p := rfl
-
-variables {m₁ m₂} (h : m₁ ≤ m₂)
-
-def cast_le (h : m₁ ≤ m₂) : subformula L m₁ n →ₗ subformula L m₂ n :=
-rew (subterm.metavar ∘ fin.cast_le h)
-
-@[simp] lemma cast_le_function {k} (r : L.pr k) (v : fin k → subterm L m₁ n) :
-  cast_le h (relation r v) = relation r (subterm.cast_le h ∘ v) :=
-by simp[cast_le]; refl
-
-@[simp] lemma cast_le_neg_function {k} (r : L.pr k) (v : fin k → subterm L m₁ n) :
-  cast_le h (neg_relation r v) = neg_relation r (subterm.cast_le h ∘ v) :=
-by simp[cast_le]; refl
-
-@[simp] lemma cast_le_fal (p : subformula L m₁ (n + 1)) :
-  cast_le h (∀'p) = ∀'(cast_le h p) :=
-by simp[cast_le]; refl
-
-@[simp] lemma cast_le_ex (p : subformula L m₁ (n + 1)) :
-  cast_le h (∃'p) = ∃'(cast_le h p) :=
-by simp[cast_le]; refl
 
 end mlift
 
 section push
 
-@[simp] def push' {m} : Π {n}, subformula L m (n + 1) → subformula L (m + 1) n
+@[simp] def push' {m} : Π {n}, bounded_subformula L m (n + 1) → bounded_subformula L (m + 1) n
 | n verum              := ⊤
 | n falsum             := ⊥
 | n (relation p v)     := relation p (subterm.push ∘ v)
@@ -206,18 +345,18 @@ section push
 | n (ex p)             := ∃'p.push'
 using_well_founded {rel_tac := λ _ _, `[exact ⟨_, measure_wf (λ x, x.2.complexity)⟩]}
 
-@[simp] lemma push'_neg : ∀ {n} (p : subformula L m (n + 1)), (∼p).push' = ∼p.push'
+@[simp] lemma push'_neg : ∀ {n} (p : bounded_subformula L m (n + 1)), (∼p).push' = ∼p.push'
 | n verum              := by simp[←falsum_eq, ←verum_eq, ←not_eq]
 | n falsum             := by simp[←falsum_eq, ←verum_eq, ←not_eq]
 | n (relation p v)     := by simp
 | n (neg_relation p v) := by simp
 | n (and p q)          := by simp[←not_eq, ←and_eq, ←or_eq]; exact ⟨push'_neg p, push'_neg q⟩
 | n (or p q)           := by simp[←not_eq, ←and_eq, ←or_eq]; exact ⟨push'_neg p, push'_neg q⟩
-| n (fal p)            := by simp[←not_eq, ←fal_eq, ←ex_eq]; exact push'_neg p
-| n (ex p)             := by simp[←not_eq, ←fal_eq, ←ex_eq]; exact push'_neg p
+| n (fal p)            := by simp[←not_eq, ←fal_eq, ←ex_eq]; rw[←fal_eq, ←ex_eq]; simp; exact push'_neg p
+| n (ex p)             := by simp[←not_eq, ←fal_eq, ←ex_eq]; rw[←fal_eq, ←ex_eq]; simp; exact push'_neg p
 using_well_founded {rel_tac := λ _ _, `[exact ⟨_, measure_wf (λ x, x.2.complexity)⟩]}
 
-def push : subformula L m (n + 1) →ₗ subformula L (m + 1) n :=
+def push : bounded_subformula L m (n + 1) →ₗ bounded_subformula L (m + 1) n :=
 { to_fun := push',
   map_neg' := λ p, by simp,
   map_imply' := λ p q, by simp[imply_def, ←or_eq],
@@ -226,23 +365,23 @@ def push : subformula L m (n + 1) →ₗ subformula L (m + 1) n :=
   map_top' := by simp[←verum_eq],
   map_bot' := by simp[←falsum_eq] }
 
-@[simp] lemma push_relation {k} (r : L.pr k) (v : fin k → subterm L m (n + 1)) :
+@[simp] lemma push_relation {k} (r : L.pr k) (v : fin k → bounded_subterm L m (n + 1)) :
   push (relation r v) = relation r (subterm.push ∘ v) := by simp[push]
 
-@[simp] lemma push_neg_relation {k} (r : L.pr k) (v : fin k → subterm L m (n + 1)) :
+@[simp] lemma push_neg_relation {k} (r : L.pr k) (v : fin k → bounded_subterm L m (n + 1)) :
   push (neg_relation r v) = neg_relation r (subterm.push ∘ v) := by simp[push]
 
-@[simp] lemma push_fal (p : subformula L m (n + 1 + 1)) :
+@[simp] lemma push_fal (p : bounded_subformula L m (n + 1 + 1)) :
   push (∀'p) = ∀'push p := by simp[push]; unfold has_univ_quantifier'.univ; simp; refl
 
-@[simp] lemma push_ex (p : subformula L m (n + 1 + 1)) :
+@[simp] lemma push_ex (p : bounded_subformula L m (n + 1 + 1)) :
   push (∃'p) = ∃'push p := by simp[push]; unfold has_exists_quantifier'.ex; simp; refl
 
 end push
 
 section pull
 
-@[simp] def pull' {m} : Π {n}, subformula L (m + 1) n → subformula L m (n + 1)
+@[simp] def pull' {m} : Π {n}, bounded_subformula L (m + 1) n → bounded_subformula L m (n + 1)
 | n verum              := ⊤
 | n falsum             := ⊥
 | n (relation p v)     := relation p (subterm.pull ∘ v)
@@ -252,10 +391,10 @@ section pull
 | n (fal p)            := ∀'p.pull'
 | n (ex p)             := ∃'p.pull'
 
-@[simp] lemma pull_neg (p : subformula L (m + 1) n) : (∼p).pull' = ∼p.pull' :=
-by induction p; simp[mlift, ←verum_eq, ←falsum_eq, ←and_eq, ←or_eq, ←not_eq, ←fal_eq, ←ex_eq, *] at*
+@[simp] lemma pull_neg (p : bounded_subformula L (m + 1) n) : (∼p).pull' = ∼p.pull' :=
+by induction p; simp[←verum_eq, ←falsum_eq, ←and_eq, ←or_eq, ←not_eq, ←fal_eq, ←ex_eq, *] at*; refl
 
-def pull : subformula L (m + 1) n →ₗ subformula L m (n + 1) :=
+def pull : bounded_subformula L (m + 1) n →ₗ bounded_subformula L m (n + 1) :=
 { to_fun := pull',
   map_neg' := λ p, by simp,
   map_imply' := λ p q, by simp[imply_def, ←or_eq],
@@ -264,66 +403,68 @@ def pull : subformula L (m + 1) n →ₗ subformula L m (n + 1) :=
   map_top' := by refl,
   map_bot' := by refl }
 
-@[simp] lemma pull_relation {k} (r : L.pr k) (v : fin k → subterm L (m + 1) n) :
+@[simp] lemma pull_relation {k} (r : L.pr k) (v : fin k → bounded_subterm L (m + 1) n) :
   pull (relation r v) = relation r (subterm.pull ∘ v) := rfl
 
-@[simp] lemma pull_neg_relation {k} (r : L.pr k) (v : fin k → subterm L (m + 1) n) :
+@[simp] lemma pull_neg_relation {k} (r : L.pr k) (v : fin k → bounded_subterm L (m + 1) n) :
   pull (neg_relation r v) = neg_relation r (subterm.pull ∘ v) := rfl
+
+@[simp] lemma pull_fal (p : bounded_subformula L (m + 1) (n + 1)) :
+  pull (∀'p) = ∀'pull p := by simp[pull]; unfold has_univ_quantifier'.univ; simp; refl
+
+@[simp] lemma pull_ex (p : bounded_subformula L (m + 1) (n + 1)) :
+  pull (∃'p) = ∃'pull p := by simp[pull]; unfold has_exists_quantifier'.ex; simp; refl
 
 end pull
 
-def msubst (t : subterm L m n) : subformula L (m + 1) n →ₗ subformula L m n :=
-rew (subterm.metavar <* t)
+section cast_le
 
-section msubst
-variables (u : subterm L m n)
+variables {m₁ m₂} (h : m₁ ≤ m₂)
 
-@[simp] lemma msubst_relation {p} (r : L.pr p) (v) :
-  msubst u (relation r v) = relation r (subterm.msubst u ∘ v) := by simp[msubst, subterm.msubst]
+def cast_le (h : m₁ ≤ m₂) : bounded_subformula L m₁ n →ₗ bounded_subformula L m₂ n :=
+map (fin.cast_le h)
 
-@[simp] lemma msubst_neg_relation {p} (r : L.pr p) (v) :
-  msubst u (neg_relation r v) = neg_relation r (subterm.msubst u ∘ v) := by simp[msubst, subterm.msubst]
+@[simp] lemma cast_le_function {k} (r : L.pr k) (v : fin k → bounded_subterm L m₁ n) :
+  cast_le h (relation r v) = relation r (λ i, subterm.cast_le h (v i)) :=
+by simp[cast_le]; refl
 
-@[simp] lemma msubst_fal (p : subformula L (m + 1) (n + 1)) :
-  msubst u (∀'p) = ∀'msubst u.lift p := by simp[msubst, fin.comp_right_concat]
+@[simp] lemma cast_le_neg_function {k} (r : L.pr k) (v : fin k → bounded_subterm L m₁ n) :
+  cast_le h (neg_relation r v) = neg_relation r (subterm.cast_le h ∘ v) :=
+by simp[cast_le]; refl
 
-@[simp] lemma msubst_ex (p : subformula L (m + 1) (n + 1)) :
-  msubst u (∃'p) = ∃'msubst u.lift p := by simp[msubst, fin.comp_right_concat]
+@[simp] lemma cast_le_fal (p : bounded_subformula L m₁ (n + 1)) :
+  cast_le h (∀'p) = ∀'(cast_le h p) :=
+by simp[cast_le]; refl
 
-end msubst
+@[simp] lemma cast_le_ex (p : bounded_subformula L m₁ (n + 1)) :
+  cast_le h (∃'p) = ∃'(cast_le h p) :=
+by simp[cast_le]; refl
 
-def subst (u : subterm L m n) : subformula L m (n + 1) →ₗ subformula L m n := (msubst u).comp push
+@[simp] lemma uniform_subst (u : bounded_subterm L m₁ n) (p : bounded_subformula L m₁ (n + 1)) :
+  cast_le h (subst u p) = subst (subterm.cast_le h u) (cast_le h p) :=
+by simp[cast_le, subterm.cast_le, map_subst]
 
-section subst
-variables (u : subterm L m n)
+variables {m₁ m₂} (f : fin (m₁ + 1) → fin m₂)
 
-@[simp] lemma subst_relation {p} (r : L.pr p) (v) :
-  subst u (relation r v) = relation r (subterm.subst u ∘ v) := by simp[subst, subterm.subst, subterm.msubst]
+@[simp] lemma cast_le_mlift (p : bounded_subformula L m₁ n) (h : m₁ + 1 ≤ m₂) :
+  cast_le h (mlift p) = cast_le (nat.le_of_succ_le h) p :=
+by simp[cast_le, mlift]; congr
 
-@[simp] lemma subst_neg_relation {p} (r : L.pr p) (v) :
-  subst u (neg_relation r v) = neg_relation r (subterm.subst u ∘ v) := by simp[subst, subterm.subst, subterm.msubst]
+@[simp] lemma mlift_cast_le (p : bounded_subformula L m₁ n) (h : m₁ ≤ m₂) :
+  mlift (cast_le h p) = cast_le (le_add_right h) p :=
+by simp[cast_le, mlift]; congr
 
-@[simp] lemma subst_fal (p : subformula L m (n + 1 + 1)) :
-  subst u (∀'p) = ∀'subst u.lift p := by simp[subst]
+lemma push_eq_subst_mlift (p : bounded_subformula L m (n + 1)) :
+  push p = subst &(fin.last m) p.mlift :=
+by apply ind_succ_on p; intros; simp*
 
-@[simp] lemma subst_ex (p : subformula L m (n + 1 + 1)) :
-  subst u (∃'p) = ∃'subst u.lift p := by simp[subst]
+@[simp] lemma uniform_push (h : m₁ + 1 ≤ m₂) (p : bounded_subformula L m₁ (n + 1)) :
+  cast_le h (push p) = subst &(fin.cast_le h $ fin.last m₁) (cast_le (nat.le_of_succ_le h) p) :=
+by simp[push_eq_subst_mlift]
 
-@[simp] lemma cast_le_subst (h : m₁ ≤ m₂) : ∀ {n} (u : subterm L m₁ n) (p : subformula L m₁ (n + 1)),
-  cast_le h (subst u p) = subst (u.cast_le h) (cast_le h p)
-| n u verum              := by simp[verum_eq]
-| n u falsum             := by simp[falsum_eq]
-| n u (relation r v)     := by simp[(∘)]
-| n u (neg_relation r v) := by simp[(∘)]
-| n u (and p q)          := by simp[and_eq]; exact ⟨cast_le_subst u p, cast_le_subst u q⟩
-| n u (or p q)           := by simp[or_eq]; exact ⟨cast_le_subst u p, cast_le_subst u q⟩
-| n u (fal p)            := by simp[fal_eq]; refine cast_le_subst u.lift p
-| n u (ex p)             := by simp[ex_eq]; refine cast_le_subst u.lift p
-using_well_founded {rel_tac := λ _ _, `[exact ⟨_, measure_wf (λ x, x.2.2.complexity)⟩]}
+end cast_le
 
-end subst
-
-@[simp] def to_fol : Π {n}, subformula L m n → fol.subformula L m n
+@[simp] def to_fol : Π {n}, subformula L μ n → fol.subformula L μ n
 | n verum              := ⊤
 | n falsum             := ⊥
 | n (relation r v)     := fol.subformula.relation r v
@@ -333,148 +474,23 @@ end subst
 | n (fal p)            := ∀'p.to_fol
 | n (ex p)             := ∃'p.to_fol
 
-@[simp] lemma to_fol_verum : to_fol (⊤ : subformula L m n) = ⊤ := rfl
+@[simp] lemma to_fol_verum : to_fol (⊤ : subformula L μ n) = ⊤ := rfl
 
-@[simp] lemma to_fol_falsum : to_fol (⊥ : subformula L m n) = ⊥ := rfl
+@[simp] lemma to_fol_falsum : to_fol (⊥ : subformula L μ n) = ⊥ := rfl
 
-@[simp] lemma to_fol_and (p q : subformula L m n) : to_fol (p ⊓ q) = to_fol p ⊓ to_fol q := rfl
+@[simp] lemma to_fol_and (p q : subformula L μ n) : to_fol (p ⊓ q) = to_fol p ⊓ to_fol q := rfl
 
-@[simp] lemma to_fol_or (p q : subformula L m n) : to_fol (p ⊔ q) = to_fol p ⊔ to_fol q := rfl
+@[simp] lemma to_fol_or (p q : subformula L μ n) : to_fol (p ⊔ q) = to_fol p ⊔ to_fol q := rfl
 
-@[simp] lemma to_fol_fal (p : subformula L m (n + 1)) : to_fol (∀'p) = ∀'to_fol p := rfl
+@[simp] lemma to_fol_fal (p : subformula L μ (n + 1)) : to_fol (∀'p) = ∀'to_fol p := rfl
 
-@[simp] lemma to_fol_ex (p : subformula L m (n + 1)) : to_fol (∃'p) = ∃'to_fol p := rfl
+@[simp] lemma to_fol_ex (p : subformula L μ (n + 1)) : to_fol (∃'p) = ∃'to_fol p := rfl
 
-end subformula
+end bounded
 
-end Tait
+section nat
 
-namespace subformula
-variables {L m n}
-
-@[simp] def to_Tait : Π {n}, subformula L m n → Tait.subformula L m n
-| n verum          := ⊤
-| n (relation r v) := Tait.subformula.relation r v
-| n (imply p q)    := p.to_Tait ⟶ q.to_Tait
-| n (neg p)        := ∼p.to_Tait
-| n (fal p)        := ∀'p.to_Tait
-
-@[simp] lemma to_Tait_verum : to_Tait (⊤ : subformula L m n) = ⊤ := rfl
-
-end subformula
-
-namespace Tait
-
-namespace subformula
-variables {L₁ L₂} (l : L₁ ⤳ᴸ L₂) {m n}
-
-@[simp] def of_lhom' : Π {n}, subformula L₁ m n → subformula L₂ m n
-| n verum              := ⊤
-| n falsum             := ⊥
-| n (relation r v)     := relation (l.pr _ r) (λ i, subterm.of_lhom l (v i))
-| n (neg_relation r v) := neg_relation (l.pr _ r) (λ i, subterm.of_lhom l (v i))
-| n (and p q)          := of_lhom' p ⊓ of_lhom' q
-| n (or p q)           := of_lhom' p ⊔ of_lhom' q
-| n (fal p)            := ∀'of_lhom' p
-| n (ex p)             := ∃'of_lhom' p
-
-@[simp] lemma of_lhom'_neg (p : subformula L₁ m n) : of_lhom' l (∼p) = ∼ of_lhom' l p :=
-by induction p; simp[mlift, ←verum_eq, ←falsum_eq, ←and_eq, ←or_eq, ←not_eq, ←fal_eq, ←ex_eq, *] at*
-
-def of_lhom : subformula L₁ m n →ₗ subformula L₂ m n :=
-{ to_fun := of_lhom' l,
-  map_neg' := λ p, by simp,
-  map_imply' := λ p q, by simp[imply_def, ←or_eq],
-  map_and' := λ p q, by refl,
-  map_or' := λ p q, by refl,
-  map_top' := by refl,
-  map_bot' := by refl }
-
-@[simp] lemma of_lhom_rel {k} (r : L₁.pr k) (v : fin k → subterm L₁ m n) :
-  of_lhom l (relation r v) = relation (l.pr k r) (λ i, subterm.of_lhom l (v i)) := rfl
-
-@[simp] lemma of_lhom_neg_rel {k} (r : L₁.pr k) (v : fin k → subterm L₁ m n) :
-  of_lhom l (neg_relation r v) = neg_relation (l.pr k r) (λ i, subterm.of_lhom l (v i)) := rfl
-
-@[simp] lemma of_lhom_fal (p : subformula L₁ m (n + 1)) : of_lhom l (∀'p) = ∀'of_lhom l p := rfl
-
-@[simp] lemma of_lhom_ex (p : subformula L₁ m (n + 1)) : of_lhom l (∃'p) = ∃'of_lhom l p := rfl
-
-end subformula
-
-variables (L)
-
-inductive uniform_subformula : ℕ → Type u
-| verum        {n} : uniform_subformula n
-| falsum       {n} : uniform_subformula n
-| relation     {n} : ∀ {p}, L.pr p → (fin p → uniform_subterm L n) → uniform_subformula n
-| neg_relation {n} : ∀ {p}, L.pr p → (fin p → uniform_subterm L n) → uniform_subformula n
-| and          {n} : uniform_subformula n → uniform_subformula n → uniform_subformula n
-| or           {n} : uniform_subformula n → uniform_subformula n → uniform_subformula n
-| fal          {n} : uniform_subformula (n + 1) → uniform_subformula n
-| ex           {n} : uniform_subformula (n + 1) → uniform_subformula n
-
-@[reducible] def uniform_formula := uniform_subformula L 0
-
-namespace uniform_subformula
-variables {L m n}
-
-instance : has_univ_quantifier' (uniform_subformula L) := ⟨@fal L⟩
-
-instance : has_exists_quantifier' (uniform_subformula L) := ⟨@ex L⟩
-
-@[simp] def not : Π {n}, Tait.uniform_subformula L n → Tait.uniform_subformula L n
-| n verum              := falsum
-| n falsum             := verum
-| n (relation r v)     := neg_relation r v
-| n (neg_relation r v) := relation r v
-| n (and p q)          := or p.not q.not
-| n (or p q)           := and p.not q.not
-| n (fal p)            := ex p.not
-| n (ex p)             := fal p.not
-
-instance : has_logic_symbol (uniform_subformula L n) := Tait.logic_simbol_default (uniform_subformula L n) verum falsum not and or
-
-lemma verum_eq : @verum L n = ⊤ := rfl
-lemma falsum_eq : @falsum L n = ⊥ := rfl
-lemma and_eq : @and L n = has_inf.inf := rfl
-lemma or_eq : @or L n = has_sup.sup := rfl
-lemma not_eq : @not L n = has_negation.neg := rfl
-lemma imply_def (p q : uniform_subformula L n) : (p ⟶ q) = (∼p) ⊔ q := by refl
-lemma fal_eq : @fal L n = has_univ_quantifier'.univ := rfl
-lemma ex_eq : @ex L n = has_exists_quantifier'.ex := rfl
-
-@[simp] lemma and.inj' (p₁ q₁ p₂ q₂ : uniform_subformula L n) : p₁ ⊓ p₂ = q₁ ⊓ q₂ ↔ p₁ = q₁ ∧ p₂ = q₂ :=
-by simp[has_inf.inf]
-
-@[simp] lemma or.inj' (p₁ q₁ p₂ q₂ : uniform_subformula L n) : p₁ ⊔ p₂ = q₁ ⊔ q₂ ↔ p₁ = q₁ ∧ p₂ = q₂ :=
-by simp[has_sup.sup]
-
-@[simp] lemma fal.inj' (p q : uniform_subformula L (n + 1)) : ∀'p = ∀'q ↔ p = q :=
-by simp[has_univ_quantifier'.univ]
-
-@[simp] lemma ex.inj' (p q : uniform_subformula L (n + 1)) : ∃'p = ∃'q ↔ p = q := 
-by simp[has_exists_quantifier'.ex]
-
-@[simp] lemma not_verum : ∼(⊤ : uniform_subformula L n) = ⊥ := by refl
-
-@[simp] lemma not_falsum : ∼(⊥ : uniform_subformula L n) = ⊤ := by refl
-
-@[simp] lemma not_relation {k} (r : L.pr k) (v : fin k → uniform_subterm L n) :
-  ∼(relation r v) = neg_relation r v := by refl
-
-@[simp] lemma not_neg_relation {k} (r : L.pr k) (v : fin k → uniform_subterm L n) :
-  ∼(neg_relation r v) = relation r v := by refl
-
-@[simp] lemma not_and (p q : uniform_subformula L n) : ∼(p ⊓ q) = ∼p ⊔ ∼q := by refl
-
-@[simp] lemma not_or (p q : uniform_subformula L n) : ∼(p ⊔ q) = ∼p ⊓ ∼q := by refl
-
-@[simp] lemma not_fal (p : uniform_subformula L (n + 1)) : ∼(∀'p) = ∃'∼p := by refl
-
-@[simp] lemma not_ex (p : uniform_subformula L (n + 1)) : ∼(∃'p) = ∀'∼p := by refl
-
-@[simp] def arity : Π {n}, Tait.uniform_subformula L n → ℕ
+@[simp] def arity : Π {n}, subformula L ℕ n → ℕ
 | n verum              := 0
 | n falsum             := 0
 | n (relation r v)     := ⨆ᶠ i, (v i).arity
@@ -484,115 +500,98 @@ by simp[has_exists_quantifier'.ex]
 | n (fal p)            := p.arity
 | n (ex p)             := p.arity
 
-@[simp] def to_subformula : ∀ {n} (p : uniform_subformula L n), p.arity ≤ m → subformula L m n
-| n verum              h := ⊤
-| n falsum             h := ⊥
-| n (relation r v)     h := subformula.relation r (λ i, (v i).to_subterm (by show (v i).arity ≤ m; simp at h; exact h i))
-| n (neg_relation r v) h := subformula.neg_relation r (λ i, (v i).to_subterm (by show (v i).arity ≤ m; simp at h; exact h i))
-| n (and p q)          h := have h : p.arity ≤ m ∧ q.arity ≤ m, by simpa using h, p.to_subformula h.1 ⊓ q.to_subformula h.2
-| n (or p q)           h := have h : p.arity ≤ m ∧ q.arity ≤ m, by simpa using h, p.to_subformula h.1 ⊔ q.to_subformula h.2
-| n (fal p)            h := ∀'p.to_subformula (by simpa using h)
-| n (ex p)             h := ∃'p.to_subformula (by simpa using h)
+@[simp] lemma arity_verum : (⊤ : subformula L ℕ n).arity = 0 := rfl
+@[simp] lemma arity_falsum : (⊥ : subformula L ℕ n).arity = 0 := rfl
+@[simp] lemma arity_and (p q : subformula L ℕ n) : (p ⊓ q).arity = max p.arity q.arity := rfl
+@[simp] lemma arity_or (p q : subformula L ℕ n) : (p ⊔ q).arity = max p.arity q.arity := rfl
+@[simp] lemma arity_fal (p : subformula L ℕ (n + 1)) : (∀'p).arity = p.arity := rfl
+@[simp] lemma arity_ex (p : subformula L ℕ (n + 1)) : (∃'p).arity = p.arity := rfl
 
-@[simp] def complexity : Π {n}, uniform_subformula L n → ℕ
-| n verum              := 0
-| n falsum             := 0
-| n (relation p v)     := 0
-| n (neg_relation p v) := 0
-| n (and p q)          := max p.complexity q.complexity + 1
-| n (or p q)           := max p.complexity q.complexity + 1
-| n (fal p)            := p.complexity + 1
-| n (ex p)             := p.complexity + 1
+@[simp] lemma arity_not (p : subformula L ℕ n) : (∼p).arity = p.arity :=
+by simp[←not_eq]; induction p; simp*
 
-section subst
+@[simp] def to_bform {m} : Π {n} (p : subformula L ℕ n), p.arity ≤ m → bounded_subformula L m n
+| n verum              h := verum
+| n falsum             h := falsum
+| n (relation r v)     h := relation r (λ i, (v i).to_bterm (by simp at h; exact h i))
+| n (neg_relation r v) h := neg_relation r (λ i, (v i).to_bterm (by simp at h; exact h i))
+| n (and p q)          h := have p.arity ≤ m ∧ q.arity ≤ m, by simpa using h, and (p.to_bform this.1) (q.to_bform this.2)
+| n (or p q)           h := have p.arity ≤ m ∧ q.arity ≤ m, by simpa using h, or (p.to_bform this.1) (q.to_bform this.2)
+| n (fal p)            h := fal (p.to_bform (by simpa using h))
+| n (ex p)             h := ex (p.to_bform (by simpa using h))
 
-@[simp] def subst' : Π {n}, uniform_subterm L n → Tait.uniform_subformula L (n + 1) → Tait.uniform_subformula L n
-| n t verum              := ⊤
-| n t falsum             := ⊥
-| n t (relation r v)     := relation r (uniform_subterm.subst t ∘ v)
-| n t (neg_relation r v) := neg_relation r (uniform_subterm.subst t ∘ v)
-| n t (and p q)          := (subst' t p) ⊓ (subst' t q)
-| n t (or p q)           := (subst' t p) ⊔ (subst' t q)
-| n t (fal p)            := ∀'(subst' t.lift p)
-| n t (ex p)             := ∃'(subst' t.lift p)
-using_well_founded {rel_tac := λ _ _, `[exact ⟨_, measure_wf (λ x, x.2.2.complexity)⟩]}
+@[simp] lemma to_bform_verum (h) : ((⊤ : subformula L ℕ n).to_bform h : bounded_subformula L m n) = ⊤ := rfl
+@[simp] lemma to_bform_falsum (h) : ((⊥ : subformula L ℕ n).to_bform h : bounded_subformula L m n) = ⊥ := rfl
+@[simp] lemma to_bform_and (p q : subformula L ℕ n) (h) : 
+  ((p ⊓ q).to_bform h : bounded_subformula L m n) = p.to_bform (by simp at h; exact h.1) ⊓ q.to_bform (by simp at h; exact h.2) := rfl
+@[simp] lemma to_bform_or (p q : subformula L ℕ n) (h) :
+  ((p ⊔ q).to_bform h : bounded_subformula L m n) = p.to_bform (by simp at h; exact h.1) ⊔ q.to_bform (by simp at h; exact h.2) := rfl
+@[simp] lemma to_bform_fal (p : subformula L ℕ (n + 1)) (h) : 
+  ((∀'p).to_bform h : bounded_subformula L m n) = ∀'p.to_bform (by simpa using h) := rfl
+@[simp] lemma to_bform_ex (p : subformula L ℕ (n + 1)) (h) :
+  ((∃'p).to_bform h : bounded_subformula L m n) = ∃'p.to_bform (by simpa using h) := rfl
 
-@[simp] lemma subst'_neg : ∀ {n} (t) (p : uniform_subformula L (n + 1)), subst' t (∼p) = ∼(subst' t p)
-| n t verum              := by simp[←not_eq]; refl
-| n t falsum             := by simp[←not_eq]; refl
-| n t (relation r v)     := by simp
-| n t (neg_relation r v) := by simp
-| n t (and p q)          := by {simp[←not_eq, ←or_eq, ←and_eq], refine ⟨subst'_neg t p, subst'_neg t q⟩ }
-| n t (or p q)           := by {simp[←not_eq, ←or_eq, ←and_eq], refine ⟨subst'_neg t p, subst'_neg t q⟩ }
-| n t (fal p)            := by { simp[←not_eq, ←fal_eq, ←ex_eq], refine subst'_neg t.lift p }
-| n t (ex p)             := by { simp[←not_eq, ←fal_eq, ←ex_eq], refine subst'_neg t.lift p }
-using_well_founded {rel_tac := λ _ _, `[exact ⟨_, measure_wf (λ x, x.2.2.complexity)⟩]}
+@[simp] lemma to_bform_not (p : subformula L ℕ n) {h} : (to_bform (∼p) h : bounded_subformula L m n) = ∼(to_bform p (by simpa using h)) :=
+by { simp[←not_eq], induction p; simp[*], 
+  case and : n p q IH₁ IH₂ { refine ⟨IH₁, IH₂⟩ },
+  case or  : n p q IH₁ IH₂ { refine ⟨IH₁, IH₂⟩ },
+  case fal : n p IH { exact IH },
+  case ex : n p IH { exact IH } }
 
-def subst (t : uniform_subterm L n) : Tait.uniform_subformula L (n + 1) →ₗ Tait.uniform_subformula L n :=
-{ to_fun := subst' t,
-  map_neg' := λ p, by simp,
-  map_imply' := λ p q, by simp[imply_def, ←or_eq],
-  map_and' := λ p q, by simp[←or_eq, ←and_eq],
-  map_or' := λ p q, by simp[←or_eq, ←and_eq],
-  map_top' := by simp[←verum_eq],
-  map_bot' := by simp[←falsum_eq] }
+end nat
 
-@[simp] lemma subst_relation (t : uniform_subterm L n) {k} (r : L.pr k) (v : fin k → uniform_subterm L (n + 1)) :
-  subst t (relation r v) = relation r (uniform_subterm.subst t ∘ v) := by simp[subst]
+end subformula
 
-@[simp] lemma subst_neg_relation (t : uniform_subterm L n) {k} (r : L.pr k) (v : fin k → uniform_subterm L (n + 1)) :
-  subst t (neg_relation r v) = neg_relation r (uniform_subterm.subst t ∘ v) := by simp[subst]
-
-@[simp] lemma subst_fal (t : uniform_subterm L n) (p : uniform_subformula L (n + 1 + 1)) :
-  subst t (∀'p) = ∀'(subst t.lift p) := by simp[subst, ←fal_eq]
-
-@[simp] lemma subst_ex (t : uniform_subterm L n) (p : uniform_subformula L (n + 1 + 1)) :
-  subst t (∃'p) = ∃'(subst t.lift p) := by simp[subst, ←ex_eq]
-
-end subst
-
-end uniform_subformula
+end Tait
 
 namespace subformula
-open uniform_subformula
+variables {L μ n}
+
+@[simp] def to_Tait : Π {n}, subformula L μ n → Tait.subformula L μ n
+| n verum          := ⊤
+| n (relation r v) := Tait.subformula.relation r v
+| n (imply p q)    := p.to_Tait ⟶ q.to_Tait
+| n (neg p)        := ∼p.to_Tait
+| n (fal p)        := ∀'p.to_Tait
+
+@[simp] lemma to_Tait_verum : to_Tait (⊤ : subformula L μ n) = ⊤ := rfl
+
+end subformula
+
+namespace Tait
+
+namespace subformula
 variables {L m n}
 
-@[simp] def uniform : Π {n}, subformula L m n → uniform_subformula L n
-| n verum              := uniform_subformula.verum
-| n falsum             := uniform_subformula.falsum
-| n (relation r v)     := uniform_subformula.relation r (subterm.uniform ∘ v)
-| n (neg_relation r v) := uniform_subformula.neg_relation r (subterm.uniform ∘ v)
-| n (and p q)          := uniform_subformula.and p.uniform q.uniform
-| n (or p q)           := uniform_subformula.or p.uniform q.uniform
-| n (fal p)            := uniform_subformula.fal p.uniform
-| n (ex p)             := uniform_subformula.ex p.uniform
+def uniform : bounded_subformula L m n →ₗ subformula L ℕ n := map coe
 
-@[simp] lemma top_uniform_verum : (⊤ : subformula L m n).uniform = uniform_subformula.verum := rfl
+@[simp] lemma uniform_inj (p q : bounded_subformula L m n) :
+  p.uniform = q.uniform ↔ p = q :=
+⟨λ h, map_inj_of_inj coe fin.coe_injective h, λ e, by simp[e]⟩
 
-@[simp] lemma top_uniform_falsum : (⊥ : subformula L m n).uniform = uniform_subformula.falsum := rfl
+@[simp] lemma uniform_relation {k} (r : L.pr k) (v : fin k → bounded_subterm L m n) :
+  uniform (relation r v) = relation r (λ i, subterm.uniform (v i)) := by simp[uniform, subterm.uniform]
 
-@[simp] lemma uniform_and (p q : subformula L m n) : (p ⊓ q).uniform = p.uniform.and q.uniform := rfl
+@[simp] lemma uniform_neg_relation {k} (r : L.pr k) (v : fin k → bounded_subterm L m n) :
+  uniform (neg_relation r v) = neg_relation r (λ i, subterm.uniform (v i)) := by simp[uniform, subterm.uniform]
 
-@[simp] lemma uniform_or (p q : subformula L m n) : (p ⊔ q).uniform = p.uniform.or q.uniform := rfl
+@[simp] lemma uniform_fal (p : bounded_subformula L m (n + 1)) :
+  uniform (∀'p) = ∀'uniform p := by simp[uniform]; unfold has_univ_quantifier'.univ; simp; refl
 
-@[simp] lemma uniform_fal (p : subformula L m (n + 1)) : (∀'p).uniform = p.uniform.fal := rfl
+@[simp] lemma uniform_ex (p : bounded_subformula L m (n + 1)) :
+  uniform (∃'p) = ∃'uniform p := by simp[uniform]; unfold has_exists_quantifier'.ex; simp; refl
 
-@[simp] lemma uniform_ex (p : subformula L m (n + 1)) : (∃'p).uniform = p.uniform.ex := rfl
+@[simp] lemma uniform_mlift (p : bounded_subformula L m n) : p.mlift.uniform = p.uniform :=
+by simp[mlift, uniform]; congr
 
-@[simp] lemma uniform_mlift (p : subformula L m n) : p.mlift.uniform = p.uniform :=
-by simp[mlift]; induction p; simp[mlift', ←fal_eq, ←verum_eq, ←falsum_eq, ←and_eq, ←or_eq, ←fal_eq, ←ex_eq, (∘), *]
+@[simp] lemma uniform_to_subterm (p : bounded_subformula L m n) (h) : to_bform p.uniform h = p :=
+by induction p using fol.Tait.subformula.ind_on; simp*
 
-@[simp] lemma uniform_to_subterm (p : subformula L m n) (h) : p.uniform.to_subformula h = p :=
-by induction p; simp*; refl
+@[simp] lemma to_subterm_uniform (p : subformula L ℕ n) (h : p.arity ≤ m) : (p.to_bform h).uniform = p :=
+by induction p using fol.Tait.subformula.ind_on; simp*
 
-@[simp] lemma to_subterm_uniform (p : uniform_subformula L n) (h : p.arity ≤ m) : (p.to_subformula h).uniform = p :=
-by induction p; simp[←fal_eq, ←verum_eq, ←falsum_eq, ←and_eq, ←or_eq, ←fal_eq, ←ex_eq, (∘), *]
-
-@[simp] lemma subformula_arity (p : subformula L m n) : p.uniform.arity ≤ m :=
-by induction p; simp*
-
-@[simp] lemma sentence_arity (σ : subformula L 0 n) : σ.uniform.arity ≤ m :=
-le_trans (subformula_arity σ) (by simp)
+@[simp] lemma subformula_arity (p : bounded_subformula L m n) : p.uniform.arity ≤ m :=
+by induction p using fol.Tait.subformula.ind_on; simp*
 
 end subformula
 
