src/QL/FOL/coding.lean
@@ -1,13 +1,13 @@
-import QL.FOL.uniform provability consistency
+import QL.FOL.fol provability consistency
 
 universes u v
 
 namespace fol
 open_locale logic_symbol
-variables (L : language.{u}) {m m₁ m₂ n : ℕ}
+variables (L : language.{u}) {μ : Type v} {m m₁ m₂ n : ℕ}
 
-namespace uniform_subterm
-variables {L n}
+namespace subterm
+variables {L μ n}
 
 section encode
 variables (L n)
@@ -21,17 +21,17 @@ def label_type : label L n → Type
 
 variables {L n}
 
-@[reducible] def W_to_subterm : W_type (label_type L n) → uniform_subterm L n
-| ⟨sum.inl x, _⟩                := uvar x
-| ⟨sum.inr $ sum.inl x, _⟩      := var x
+@[reducible] def W_to_subterm : W_type (label_type L n) → subterm L ℕ n
+| ⟨sum.inl x, _⟩                := &x
+| ⟨sum.inr $ sum.inl x, _⟩      := #x
 | ⟨sum.inr $ sum.inr ⟨k, f⟩, F⟩ := function f (λ x, W_to_subterm (F x))
 
-def subterm_to_W : uniform_subterm L n → W_type (label_type L n)
-| &&x       := ⟨sum.inl x, empty.rec _⟩
-| (var x)        := ⟨sum.inr $ sum.inl x, empty.rec _⟩
+def subterm_to_W : subterm L ℕ n → W_type (label_type L n)
+| &x             := ⟨sum.inl x, empty.rec _⟩
+| #x             := ⟨sum.inr $ sum.inl x, empty.rec _⟩
 | (function f v) := ⟨sum.inr $ sum.inr ⟨_, f⟩, λ i, subterm_to_W (v i)⟩
 
-def formula_equiv_W : uniform_subterm L n ≃ W_type (label_type L n) :=
+def formula_equiv_W : subterm L ℕ n ≃ W_type (label_type L n) :=
 { to_fun := subterm_to_W,
   inv_fun := W_to_subterm,
   left_inv := by intros p; induction p; simp[subterm_to_W, W_to_subterm, *],
@@ -50,147 +50,71 @@ instance : Π i, encodable (label_type L n i)
 | (sum.inr $ sum.inl x)      := show encodable empty, from is_empty.to_encodable
 | (sum.inr $ sum.inr ⟨k, f⟩) := fin.encodable k
 
-variables [∀ k, encodable (L.fn k)]
-
-instance : encodable (label L n) := sum.encodable
+instance [∀ k, encodable (L.fn k)] : encodable (label L n) := sum.encodable
 
 @[irreducible]
-instance : encodable (uniform_subterm L n) := encodable.of_equiv (W_type (label_type L n)) formula_equiv_W
+instance [∀ k, encodable (L.fn k)] : encodable (subterm L ℕ n) := encodable.of_equiv (W_type (label_type L n)) formula_equiv_W
 
-end encode
+--variables [encodable μ]
 
-end uniform_subterm
+@[simp] def arity : subterm L ℕ n → ℕ
+| &x             := x + 1
+| #x             := 0
+| (function f v) := ⨆ᶠ i, (v i).arity
 
-namespace subterm
-open uniform_subterm
-variables {L m n}
+@[simp] def to_bterm {m} : Π t : subterm L ℕ n, t.arity ≤ m → bounded_subterm L m n
+| &x             h := &⟨x, h⟩
+| #x             h := #x
+| (function f v) h := function f (λ i, (v i).to_bterm (by simp at h; refine h i))
 
-section encode
+def uniform : bounded_subterm L m n → subterm L ℕ n := map coe
 
-variables [∀ k, encodable (L.fn k)]
+def to_nat [∀ k, encodable (L.fn k)] : bounded_subterm L m n → ℕ := λ t, encodable.encode t.uniform
 
-def to_nat : subterm L m n → ℕ := λ t, encodable.encode t.uniform
+@[simp] lemma map_val_mlift (t : bounded_subterm L m n) : t.mlift.uniform = t.uniform :=
+by simp[uniform, mlift, (∘)]
 
-variables (L m n)
+@[simp] lemma uniform_cast_le (h : m₁ ≤ m₂) (t : bounded_subterm L m₁ n) : (cast_le h t).uniform = t.uniform :=
+by simp[cast_le, uniform, (∘)]
 
-def of_nat : ℕ → option (subterm L m n) := λ i,
-  let t := encodable.decode (uniform_subterm L n) i in
-  t.bind (λ t, if h : t.arity ≤ m then some (t.to_subterm h) else none)
+@[simp] lemma uniform_to_bform (t : bounded_subterm L m n) (h) : t.uniform.to_bterm h = t :=
+by induction t; simp[uniform, *]; case function : k f v IH { funext i, simp[uniform] at h, exact IH i (h i) }
+
+@[simp] lemma to_subterm_uniform (t : subterm L ℕ n) (h : t.arity ≤ m) : (t.to_bterm h).uniform = t :=
+by induction t; simp[uniform, *]; case function : k f v IH { funext i, simp[uniform] at h, exact IH i (h i) }
+
+@[simp] lemma subterm_arity (t : bounded_subterm L m n) : t.uniform.arity ≤ m :=
+by { induction t; simp[*, uniform], case metavar : i { exact nat.succ_le_iff.mpr i.property },
+     case function : k f v IH { simpa using IH } }
+
+@[simp] lemma uniform_push (t : bounded_subterm L m (n + 1)) :
+  (push t).uniform = subst &m t.uniform :=
+by { induction t; simp[*, uniform],
+     case var : x { refine fin.last_cases _ _ x; simp },
+     case function : k f v IH { funext i, exact IH i } }
+
+variables (L m n) [∀ k, encodable (L.fn k)]
+
+def of_nat : ℕ → option (bounded_subterm L m n) := λ i,
+  (encodable.decode (subterm L ℕ n) i).bind (λ t, if h : t.arity ≤ m then some (t.to_bterm h) else none)
 
 variables {L m m₁ m₂ n}
 
-@[simp] lemma to_nat_of_nat (t : subterm L m n) : of_nat L m n t.to_nat = some t :=
+@[simp] lemma to_nat_of_nat (t : bounded_subterm L m n) : of_nat L m n t.to_nat = some t :=
 by simp[to_nat, of_nat]
 
-@[simp] lemma of_nat_mlift (t : subterm L m n) : to_nat t.mlift = to_nat t :=
+@[simp] lemma of_nat_mlift (t : bounded_subterm L m n) : to_nat t.mlift = to_nat t :=
 by simp[to_nat]
 
-@[simp] lemma of_nat_cast_le (h : m₁ ≤ m₂) (t : subterm L m₁ n) : to_nat (t.cast_le h) = to_nat t :=
+@[simp] lemma of_nat_cast_le (h : m₁ ≤ m₂) (t : bounded_subterm L m₁ n) : to_nat (cast_le h t) = to_nat t :=
 by simp[to_nat]
+
+@[simp] lemma to_nat_to_subterm (t : subterm L ℕ n) {m} (h : t.arity ≤ m) :
+  (t.to_bterm h).to_nat = encodable.encode t :=
+by simp[subterm.to_nat]
 
 end encode
 
 end subterm
-
-namespace uniform_subterm
-variables {L n} [∀ k, encodable (L.fn k)]
-
-@[simp] lemma to_nat_to_subterm (t : uniform_subterm L n) {m} (h : t.arity ≤ m) :
-  (t.to_subterm h).to_nat = encodable.encode t :=
-by simp[subterm.to_nat]
-
-end uniform_subterm
-
-namespace uniform_subformula
-variables {L n}
-
-section encode
-open encodable nat
-variables {L n} [∀ k, encodable (L.pr k)] [∀ k, encodable (L.fn k)]
-
-@[simp] def to_nat : Π {n}, uniform_subformula L n → ℕ
-| n verum                 := 0
-| n (@relation L _ k r v) := (bit0 $ bit0 $ mkpair k $ mkpair (encode r) (encode v)) + 1
-| n (imply p q)           := (bit0 $ bit1 $ mkpair p.to_nat q.to_nat) + 1
-| n (neg p)               := (bit1 $ bit0 p.to_nat) + 1
-| n (fal p)               := (bit1 $ bit1 p.to_nat) + 1
-
-variables (L n)
-
-@[simp] def of_nat : Π n, ℕ → option (uniform_subformula L n)
-| n 0 := some verum
-| n (e + 1) :=
-    let i := e.div2.div2 in
-    have div8 : i ≤ e := by simp[i, nat.div2_val]; exact le_trans (nat.div_le_self (e/2) 2) (nat.div_le_self e 2),
-    have hi : i < e + 1, from lt_succ_iff.mpr div8,
-    have hi1 : i.unpair.1 < e + 1, from nat.lt_succ_iff.mpr (le_trans (nat.unpair_left_le _) div8),
-    have hi2 : i.unpair.2 < e + 1, from nat.lt_succ_iff.mpr (le_trans (nat.unpair_right_le _) div8),
-    match e.bodd, e.div2.bodd with
-    | ff, ff :=
-        let k := i.unpair.1,
-            r := decode (L.pr k) i.unpair.2.unpair.1,
-            v := decode (fin k → uniform_subterm L n) i.unpair.2.unpair.2 in
-      r.bind (λ r, v.map (relation r))
-    | ff, tt := (of_nat n i.unpair.1).bind (λ p, (of_nat n i.unpair.2).map (imply p))
-    | tt, ff := (of_nat n i).map neg
-    | tt, tt := (of_nat (n + 1) i).map fal
-    end
-using_well_founded {rel_tac := λ _ _, `[exact ⟨_, measure_wf (λ x, x.2)⟩]}
-
-@[simp] lemma of_nat_to_nat : ∀ {n} (p : uniform_subformula L n), of_nat L n p.to_nat = some p
-| n verum                 := by simp
-| n (@relation L _ k r v) :=
-    begin
-      simp only [to_nat, of_nat, of_nat._match_1, nat.bodd_bit0, nat.div2_bit0, nat.unpair_mkpair, encodek],
-      rw[show (unpair (mkpair k (mkpair (encode r) (encode v)))).fst = k, by simp],
-      simp only [encodek, option.some_bind', option.map_some', heq.refl], simp
-    end
-| n (imply p q)           := by simp; refine ⟨of_nat_to_nat p, of_nat_to_nat q⟩
-| n (neg p)               := by simp; refine (of_nat_to_nat p)
-| n (fal p)               := by simp; refine (of_nat_to_nat p)
-
-instance (n) : encodable (uniform_subformula L n) :=
-{ encode := to_nat,
-  decode := of_nat L n,
-  encodek := by simp }
-
-end encode
-
-end uniform_subformula
-
-namespace subformula
-open uniform_subformula
-variables {L m n}
-
-section encode
-variables [∀ k, encodable (L.fn k)] [∀ k, encodable (L.pr k)]
-
-def to_nat : subformula L m n → ℕ := λ p, encodable.encode p.uniform
-
-variables (L m n)
-
-def of_nat : ℕ → option (subformula L m n) := λ i,
-  let p := encodable.decode₂ (uniform_subformula L n) i in
-  p.bind (λ p, if h : p.arity ≤ m then some (p.to_subformula h) else none)
-
-variables {L m n}
-
-@[simp] lemma subformula_arity (p : subformula L m n) : p.uniform.arity ≤ m :=
-by induction p; simp*
-
-@[simp] lemma to_nat_of_nat (p : subformula L m n) : of_nat L m n p.to_nat = some p :=
-by simp[to_nat, of_nat]
-
-lemma of_nat_eq_some {e} {p : subformula L m n} : of_nat L m n e = some p ↔ p.to_nat = e :=
-by { simp[of_nat, to_nat, encodable.decode₂_eq_some, dite_eq_iff], split,
-  { simp, rintros _ rfl h rfl, simp },
-  { rintros rfl, refine ⟨p.uniform, rfl, by simp⟩ } }
-
-@[simp] lemma of_nat_to_nat (p : subformula L m n) : to_nat p.mlift = to_nat p :=
-by simp[to_nat]
-
-end encode
-
-end subformula
 
 end fol
